Improve definterp example based on Arjen's comments.

examples/definterp.v
@@ -13,19 +13,23 @@
   Interpreters for Imperative Languages", Poulsen, Rouvoet, Tolmach,
   Krebbers and Visser. POPL'18.
 
-  It uses well-typed and well-scoped syntax and an indexed monad to
-  define an interpreter for an imperative programming language.
+  It uses well-typed and well-scoped syntax and an monad indexed over an
+  indexed set of stores to define an interpreter for an imperative
+  programming language.
 
-  This showcases the use of dependent pattern-matching and pattern-matching
-  lambdas in Equations. We implement a variant where store extension is
-  resolved using type class resolution as well as the dependent-passing
-  style version. *)
+  This showcases the use of dependent pattern-matching and
+  pattern-matching lambdas in Equations. We implement a variant where
+  store extension is resolved using type class resolution as well as the
+  dependent-passing style version. *)
 
 Require Import Program.Basics Program.Tactics.
 From Equations Require Import Equations.
 Require Import Coq.Vectors.VectorDef.
 Require Import List.
 Import ListNotations.
+Require Import Utf8.
+Notation "( x , .. , y , z )" := (sigmaI _ x .. (sigmaI _ y z) ..) : core_scope.
+
 Set Equations Transparent.
 
 (** [t] is just [Vector.t] here. *)
@@ -95,14 +99,6 @@ Section MapAll.
   map_all_in f (all_cons p ps) := all_cons (f _ here p) (map_all_in (fun x inl => f x (there inl)) ps).
 End MapAll.
 
-Section AllSize.
-  Context {A} (P : A -> Type) (size : forall {x : A}, P x -> nat).
-
-  Equations all_size {l : list A} : All P l -> nat :=
-  all_size all_nil := 0;
-  all_size (all_cons p ps) := size _ p + all_size ps.
-End AllSize.
-
 Definition StoreTy := list Ty.
 
 Inductive Val : Ty -> StoreTy -> Set :=
@@ -136,46 +132,42 @@ Import Sigma_Notations.
 Definition store_incl (Σ Σ' : StoreTy) := &{ Σ'' : _ & Σ' = Σ'' ++ Σ }.
 Infix "⊑" := store_incl (at level 10).
 
-Lemma app_assoc {A} (x y z : list A) : x ++ y ++ z = (x ++ y) ++ z.
-Proof. induction x; simpl; auto.
-       now rewrite IHx.
-Defined.
+Equations app_assoc {A} (x y z : list A) : x ++ y ++ z = (x ++ y) ++ z :=
+  app_assoc nil y z := eq_refl;
+  app_assoc (cons x xs) y z := f_equal (cons x) (app_assoc xs y z).
 
 Section StoreIncl.
-  Context {Σ Σ' : StoreTy} (incl : Σ ⊑ Σ').
+  Equations pres_in {Σ Σ'} (incl : Σ ⊑ Σ') t (p : t ∈ Σ) : t ∈ Σ' :=
+    pres_in (Σ'', eq_refl) t p := aux Σ''
+       where aux Σ'' : t ∈ (Σ'' ++ Σ) :=
+       aux nil := p;
+       aux (cons ty tys) := there (aux tys).
 
-  Lemma pres_in t : t ∈ Σ -> t ∈ Σ'.
-  Proof. destruct incl. subst. clear. induction pr1. intros. exact H.
-         intros H. specialize (IHpr1 H). constructor 2. apply IHpr1.
-  Defined.
+  Equations refl_incl {Σ} : Σ ⊑ Σ := refl_incl := ([], eq_refl).
+
+  Equations trans_incl {Σ Σ' Σ''} (incl : Σ ⊑ Σ') (incl' : Σ' ⊑ Σ'') : Σ ⊑ Σ'' :=
+    trans_incl (p, eq_refl) (q, eq_refl) := (q ++ p, app_assoc _ _ _).
+
+  Equations store_ext_incl {Σ t} : Σ ⊑ (t :: Σ) :=
+    store_ext_incl := ([t], eq_refl).
+
+  Context {Σ Σ'} (incl : Σ ⊑ Σ').
 
   Equations weaken_val {t} (v : Val t Σ) : Val t Σ' := {
    weaken_val (@val_unit ?(Σ)) := val_unit;
    weaken_val val_true := val_true;
    weaken_val val_false := val_false;
    weaken_val (val_closure b e) := val_closure b (weaken_vals e);
-   weaken_val (val_loc H) := val_loc (pres_in _ H) }
+   weaken_val (val_loc H) := val_loc (pres_in incl _ H) }
   where weaken_vals {l} (a : All (fun t => Val t Σ) l) : All (fun t => Val t Σ') l :=
   weaken_vals all_nil := all_nil;
   weaken_vals (all_cons p ps) := all_cons (weaken_val p) (weaken_vals ps).
 
-  Lemma weakenv_vals {l} a : @weaken_vals l a = map_all (fun t v => weaken_val v) a.
-  Proof. induction a; simpl; reflexivity. Defined.
+  Equations weakenv_vals {l} a : @weaken_vals l a = map_all (fun t v => weaken_val v) a :=
+    weakenv_vals all_nil := eq_refl;
+    weakenv_vals (all_cons p ps) := f_equal (all_cons (weaken_val p)) (weakenv_vals ps).
 
-  Definition weaken_env {Γ} (v : Env Γ Σ) : Env Γ Σ' :=
-    map_all (@weaken_val) v.
-
-  Lemma refl_incl : Σ ⊑ Σ.
-  Proof. exists []. reflexivity. Defined.
-
-  Lemma trans_incl {Σ''} (incl' : Σ' ⊑ Σ'') : Σ ⊑ Σ''.
-  Proof.
-    destruct incl as [? ->], incl' as [? ->].
-    exists (pr0 ++ pr1). now rewrite app_assoc.
-  Defined.
-
-  Lemma store_ext_incl {t} : Σ ⊑ (t :: Σ).
-  Proof. now exists [t]. Defined.
+  Definition weaken_env {Γ} (v : Env Γ Σ) : Env Γ Σ' := map_all (@weaken_val) v.
 
 End StoreIncl.
 
@@ -183,9 +175,6 @@ Infix "⊚" := trans_incl (at level 10).
 
 Equations M : forall (Γ : Ctx) (P : StoreTy -> Type) (Σ : StoreTy), Type :=
   M Γ P Σ := forall (E : Env Γ Σ) (μ : Store Σ), option &{ Σ' : _ & &{ _ : Store Σ' & &{ _ : P Σ' & Σ ⊑ Σ'}}}.
-
-Require Import Utf8.
-Notation "( x , .. , y , z )" := (sigmaI _ x .. (sigmaI _ y z) ..) : core_scope.
 
 Equations bind {Σ Γ} {P Q : StoreTy -> Type} (f : M Γ P Σ) (g : ∀ {Σ'}, P Σ' -> M Γ Q Σ') : M Γ Q Σ :=
   bind f g E μ with f E μ :=
@@ -237,27 +226,21 @@ Arguments storepred_pair {P Q Σ}.
 Class Weakenable (P : StoreTy -> Type) : Type :=
   weaken : forall {Σ Σ'}, Σ ⊑ Σ' -> P Σ -> P Σ'.
 
-Instance val_weaken {t} : Weakenable (Val t).
-Proof. intros Σ Σ' incl. apply (weaken_val incl). Defined.
-
-Instance env_weaken {Γ} : Weakenable (Env Γ).
-Proof. intros Σ Σ' incl. apply (weaken_env incl). Defined.
-
-Instance loc_weaken (t : Ty) : Weakenable (In t).
-Proof. intros Σ Σ' incl. apply (pres_in incl). Defined.
+Instance val_weaken {t} : Weakenable (Val t) := fun Σ Σ' incl => weaken_val incl.
+Instance env_weaken {Γ} : Weakenable (Env Γ) := fun Σ Σ' incl => weaken_env incl.
+Instance loc_weaken (t : Ty) : Weakenable (In t) := fun Σ Σ' incl => pres_in incl t.
 
 Class IsIncludedOnce (Σ Σ' : StoreTy) : Type := is_included_once : Σ ⊑ Σ'.
 Hint Mode IsIncludedOnce + + : typeclass_instances.
 
-Instance IsIncludedOnce_ext {T} Σ : IsIncludedOnce Σ (T :: Σ).
-Proof. apply store_ext_incl. Defined.
+Instance IsIncludedOnce_ext {T} Σ : IsIncludedOnce Σ (T :: Σ) := store_ext_incl.
 
 Class IsIncluded (Σ Σ' : StoreTy) : Type := is_included : Σ ⊑ Σ'.
 Hint Mode IsIncluded + + : typeclass_instances.
 
 Instance IsIncluded_refl Σ : IsIncluded Σ Σ := refl_incl.
-Instance IsIncluded_trans Σ Σ' Σ'' : IsIncludedOnce Σ Σ' -> IsIncluded Σ' Σ'' -> IsIncluded Σ Σ''.
-Proof. intros H H'. exact (trans_incl H H'). Defined.
+Instance IsIncluded_trans Σ Σ' Σ'' : IsIncludedOnce Σ Σ' -> IsIncluded Σ' Σ'' -> IsIncluded Σ Σ'' :=
+  fun H H' => trans_incl H H'.
 
 Equations wk {Σ Σ' P} {W : Weakenable P} (p : P Σ) {incl : IsIncluded Σ Σ'} : P Σ' :=
   wk p := weaken incl p.
@@ -282,7 +265,7 @@ Equations eval_ext (n : nat) {Γ Σ t} (e : Expr Γ t) : M Γ (Val t) Σ :=
   eval_ext (S k) (var x)      := getEnv >>=' fun {Σ ext} E => ret (lookup E x);
   eval_ext (S k) (abs x)      := getEnv >>=' fun {Σ ext} E => ret (val_closure x E);
   eval_ext (S k) (app (Γ:=Γ) e1 e2) :=
-      eval_ext k e1 >>=' λ{ | _ | ext | val_closure e' E => 
+      eval_ext k e1 >>=' λ{ | _ | ext | val_closure e' E =>
       eval_ext k e2 >>=' fun {Σ' ext'} v => usingEnv (all_cons v (wk E)) (eval_ext k e')};
   eval_ext (S k) (new e)      := eval_ext k e >>=' fun {Σ ext} v => storeM v;
   eval_ext (S k) (deref l)    := eval_ext k l >>=' λ{ | _ | ext | val_loc l => derefM l };
@@ -309,7 +292,7 @@ Equations eval (n : nat) {Γ Σ t} (e : Expr Γ t) : M Γ (Val t) Σ :=
 
   eval (S k) (var x)      := getEnv >>= fun Σ E => ret (lookup E x);
   eval (S k) (abs x)      := getEnv >>= fun Σ E => ret (val_closure x E);
-  eval (S k) (app (Γ:=Γ) e1 e2) :=
+  eval (S k) (app e1 e2) :=
       eval k e1 >>= λ{ | _ | val_closure e' E =>
                              (eval k e2 ^ E) >>= fun Σ' '(storepred_pair v E) => usingEnv (all_cons v E) (eval k e')};
   eval (S k) (new e)      := eval k e >>= fun Σ v => storeM v;
@@ -331,6 +314,15 @@ Definition neg : Expr [] (bool ⇒ bool) :=
 
 Definition letref {t u} (v : Expr [] t) (b : Expr [ref t] u) : Expr [] u :=
   app (abs b) (new v).
+Obligation Tactic := idtac.
+
+Equations in_app_weaken {Σ Σ' Σ'' : StoreTy} {t} (p : t ∈ (Σ ++ Σ'')) : t ∈ (Σ ++ Σ' ++ Σ'') by struct Σ :=
+  in_app_weaken (Σ:=nil) p := pres_in (Σ', eq_refl) t p;
+  in_app_weaken (Σ:=cons _ tys) here := here;
+  in_app_weaken (Σ:=cons _ tys) (there p) := there (in_app_weaken p).
+
+Equations pres_in_prefix {Σ Σ' Σ''} (incl : Σ' ⊑ Σ'') {t} (p : t ∈ (Σ ++ Σ')) : t ∈ (Σ ++ Σ'') :=
+  pres_in_prefix (Σ'', eq_refl) p := in_app_weaken p.
 
 (** [Equations?] enters refinement mode, which can be used to solve the case of variables in proof mode. *)
 Equations? weaken_expr {Γ Γ' t u} (e1 : Expr (Γ ++ Γ') t) : Expr (Γ ++ u :: Γ') t :=
@@ -345,9 +337,7 @@ Equations? weaken_expr {Γ Γ' t u} (e1 : Expr (Γ ++ Γ') t) : Expr (Γ ++ u ::
   weaken_expr (deref l)       := deref (weaken_expr l);
   weaken_expr (assign l e)    := assign (weaken_expr l) (weaken_expr e).
 Proof.
-  clear weaken_expr.
-  induction Γ in Γ', u, x |- *. now apply there. simpl.
-  depelim x. constructor. apply there. apply IHΓ. apply x.
+  clear weaken_expr. apply (pres_in_prefix (Σ' := Γ') ([u], eq_refl) x).
 Defined.
 
 Definition seq {Γ u} (e1 : Expr Γ unit) (e2 : Expr Γ u) : Expr Γ u :=
